src/Config.fsti
@@ -45,6 +45,25 @@ val sc_selection : sc_selection_f
 inline_for_extraction
 val enable_sc_fast_selection: bool
 
+// lemmas useful for realloc optimization
+val sc_selection_is_exact1 (k:nat)
+  : Lemma
+  (requires enable_sc_fast_selection /\
+    k < US.v nb_size_classes
+  )
+  (ensures
+    US.v (sc_selection (L.index sc_list k)) == k
+  )
+
+val sc_selection_is_exact2 (k:nat)
+  : Lemma
+  (requires enable_sc_fast_selection /\
+    k < US.v nb_size_classes
+  )
+  (ensures
+    US.v (sc_selection (U32.sub (L.index sc_list k) 2ul)) == k
+  )
+
 /// Number of arenas
 inline_for_extraction
 [@ CMacro ]
